Refactoring some "basic" logic about swapping strings and the "new" operator into the theory basic_swap.  Also cleaned up a number of proofs in term_posns to better exploit the BVC-compatible structural induction principle for lambda-terms.

examples/lambda/NEWLib.sml
@@ -1,16 +1,7 @@
 structure NEWLib :> NEWLib =
 struct
 
-open HolKernel Parse boolLib BasicProvers simpLib
-open ncTheory
-
-val FRESH_STRING = prove(
-  ``!X Y. FINITE (X:string set) /\ Y SUBSET X ==> ~(NEW X IN Y)``,
-  PROVE_TAC [pred_setTheory.SUBSET_DEF, dBTheory.NEW_FRESH_string]);
-
-val FRESH_STRING_eq = prove(
-  ``!X x. FINITE (X:string set) /\ x IN X ==> ~(NEW X = x)``,
-  PROVE_TAC [pred_setTheory.SUBSET_DEF, dBTheory.NEW_FRESH_string]);
+open HolKernel boolLib BasicProvers simpLib basic_swapTheory
 
 val string_ty = stringSyntax.string_ty
 val strset_finite_t = inst [alpha |-> string_ty] pred_setSyntax.finite_tm
@@ -20,7 +11,7 @@ fun NEW_TAC vname t (asl, g) = let
   val fresh_thm =
       (CONV_RULE (RAND_CONV (REWRITE_CONV [IN_INSERT, IN_UNION, DE_MORGAN_THM,
                                            NOT_IN_EMPTY])) o
-       SPEC t) dBTheory.FRESH_string
+       SPEC t) new_exists
   fun is_finitestrset t = free_in strset_finite_t t
   val finite_asms = filter is_finitestrset asl
   val finiteness_discharged0 =
@@ -39,7 +30,7 @@ fun NEW_ELIM_TAC (asl, w) = let
   val newt = find_term (can (match_term ``NEW (X:string set)``)) w
 in
   CONV_TAC (UNBETA_CONV newt) THEN MATCH_MP_TAC NEW_ELIM_RULE THEN
-  SIMP_TAC (srw_ss()) [FINITE_FV]
+  SIMP_TAC (srw_ss()) []
 end (asl, w)
 
 end (* struct *)
